ulib/FStar.HyperStackNG.fst
@@ -1,0 +1,274 @@
+module FStar.HyperStackNG
+include FStar.HyperStack
+
+module HH = FStar.HyperHeap
+
+noeq type object : Type =
+| ObjectReference:
+    (ty: Type) ->
+    (r: reference ty) ->
+    object
+| ObjectRegionLiveness (* change "live_region" *) :
+    (r: HH.rid) ->
+    object
+
+unfold
+let objects_disjoint (o1 o2: object): Tot Type0 =
+  match o1 with
+  | ObjectReference _ r1 ->
+    begin match o2 with
+    | ObjectReference _ r2 ->
+      frameOf r1 <> frameOf r2 \/
+      (
+	frameOf r1 == frameOf r2 /\
+	~ (as_ref r1 === as_ref r2)
+      )
+    | _ -> True
+    end
+  | ObjectRegionLiveness r1 ->
+    begin match o2 with
+    | ObjectRegionLiveness r2 -> r1 <> r2
+    | _ -> True
+    end
+
+unfold
+let object_live (m: mem) (o: object): Tot Type0 =
+  match o with
+  | ObjectReference _ r -> contains m r
+  | ObjectRegionLiveness r -> live_region m r
+
+unfold
+let object_contains = object_live
+
+unfold
+let object_preserved (o: object) (m m': mem): Tot Type0 =
+  match o with
+  | ObjectReference _ r ->
+    contains m r ==> (contains m' r /\ sel m' r == sel m r)
+  | ObjectRegionLiveness r ->
+    live_region m r ==> live_region m' r
+
+unfold
+let object_includes (o1 o2: object) : Tot Type0 = o1 == o2
+
+let root_class: Modifies.class' u#0 u#1 mem 0 object =
+  Modifies.Class
+    (* heap  *)                 mem
+    (* level *)                 0
+    (* carrier *)               object
+    (* disjoint *)              objects_disjoint
+    (* live *)                  object_live
+    (* contains *)              object_contains
+    (* preserved *)             object_preserved
+    (* includes *)              object_includes
+    (* ancestor_count *)        (fun x -> 0)
+    (* ancestor_types *)        (fun x y -> false_elim ())
+    (* ancestor_class_levels *) (fun x y -> false_elim ())
+    (* ancestor_classes *)      (fun x y -> false_elim ())
+    (* ancestor_objects *)      (fun x y -> false_elim ())
+
+abstract
+let class_invariant
+  ()
+: Lemma
+  (requires True)
+  (ensures (Modifies.class_invariant root_class root_class))
+//  [SMTPat (Modifies.class_invariant root_class root_class)]
+= let s: Modifies.class_invariant_body u#0 u#1 root_class root_class = {
+    Modifies.preserved_refl =  (fun _ _ -> ());
+    Modifies.preserved_trans = (fun _ _ _ _ -> ());
+    Modifies.preserved_ancestors_preserved = begin
+      let g
+        (x: object)
+	(h: mem)
+	(h' : mem)
+	(s: squash (Modifies.Class?.ancestor_count root_class x > 0))
+	(f: (
+	  (i: nat { i < Modifies.Class?.ancestor_count root_class x } ) ->
+	  Lemma
+	  (Modifies.Class?.preserved (Modifies.Class?.ancestor_classes root_class x i) (Modifies.ancestor_objects root_class x i) h h')
+	))
+      : Lemma
+	(ensures (Modifies.Class?.preserved root_class x h h'))
+      = ()
+      in
+      g
+    end;
+    Modifies.disjoint_sym = (fun _ _ -> ());
+    Modifies.level_0_class_eq_root = ();
+    Modifies.level_0_fresh_disjoint = (fun _ _ _ _ -> ());
+    Modifies.preserved_live = (fun _ _ _ -> ());
+    Modifies.preserved_contains = (fun _ _ _ -> ());
+    Modifies.live_contains = (fun _ _ -> ());
+    Modifies.ancestors_contains = begin
+      let g
+	(h: mem)
+	(o: object)
+	(s: squash (Modifies.Class?.ancestor_count root_class o > 0))
+	(f: (
+	  (i: nat {i < Modifies.Class?.ancestor_count root_class o } ) ->
+	  Lemma
+	  (Modifies.Class?.contains (Modifies.Class?.ancestor_classes root_class o i) h (Modifies.ancestor_objects root_class o i))
+	))
+      : Lemma
+	(ensures (Modifies.Class?.contains root_class h o))
+      = ()
+      in
+      g
+    end;
+    Modifies.live_ancestors = (fun _ _ _ -> ());
+    Modifies.includes_refl = (fun _ -> ());
+    Modifies.includes_trans = (fun _ _ _ -> ());
+    Modifies.preserved_includes = (fun _ _ _ _ -> ());
+    Modifies.includes_contains = (fun _ _ _ -> ());
+    Modifies.contains_live = (fun _ _ _ -> ());
+    Modifies.includes_ancestors = (fun _ _ _ -> ());
+    Modifies.disjoint_includes = (fun _ _ _ -> ());
+  }
+  in
+  (Modifies.class_invariant_intro s)
+
+let class: Modifies.class root_class 0 object = class_invariant () ; root_class
+
+(*
+let class_eq
+  ()
+: Lemma
+  (requires True)
+  (ensures (class == root_class))
+  [SMTPatOr [[SMTPat class]; [SMTPat root_class]]]
+= ()
+*)
+
+let locset_of_reference
+  (#t: Type)
+  (r: reference t)
+: Tot (Modifies.locset u#0 u#1 root_class)
+= Modifies.locset_of_object class (ObjectReference t r)
+
+unfold
+let object_is_reference_of_region
+  (o': object)
+  (r: HH.rid)
+: Tot Type0
+= match o' with
+  | ObjectReference _ re -> frameOf re == r
+  | _ -> False
+
+assume val locset_of_region (r: HH.rid): Tot (Modifies.locset u#0 u#1 root_class)
+
+assume val mem_locset_of_region
+  (r: HH.rid)
+  (o: Modifies.loc root_class)
+: Lemma
+  (requires True)
+  (ensures (TSet.mem o (locset_of_region r) <==> (
+    exists (o' : object) .
+      o == Modifies.loc_of_object class o' /\
+      o' `object_is_reference_of_region` r
+  )))
+//  [SMTPat (TSet.mem o (locset_of_region r))]
+
+let locset_of_reference_subset_locset_of_region
+  (#t: Type)
+  (reg: HH.rid)
+  (ref: reference t)
+: Lemma
+  (requires (frameOf ref == reg))
+  (ensures (locset_of_reference ref `TSet.subset` locset_of_region reg))
+  [SMTPatOr [[SMTPatT (frameOf ref == reg)]; [SMTPat (locset_of_reference ref `TSet.subset` locset_of_region reg)]]]
+= Classical.forall_intro (mem_locset_of_region reg)
+
+let locset_of_region_liveness_tag
+  (r: HH.rid)
+: Tot (Modifies.locset u#0 u#1 root_class)
+= Modifies.locset_of_object class (ObjectRegionLiveness r)
+
+let locset_of_region_with_liveness
+  (r: HH.rid)
+: Tot (Modifies.locset u#0 u#1 root_class)
+= TSet.union (locset_of_region r) (locset_of_region_liveness_tag r)
+
+let locset_of_region_subset_locset_of_region_with_liveness
+  (r: HH.rid)
+: Lemma
+  (requires True)
+  (ensures (locset_of_region r `TSet.subset` locset_of_region_with_liveness r))
+= ()
+
+let locset_of_region_with_liveness_disjoint
+  (#t: Type)
+  (reg1 reg2: HH.rid)
+: Lemma
+  (requires (reg1 <> reg2))
+  (ensures (Modifies.locset_disjoint u#0 u#1 (locset_of_region_with_liveness reg1) (locset_of_region_with_liveness reg2)))
+  [SMTPat (reg1 <> reg2)]
+= Classical.forall_intro (mem_locset_of_region reg1);
+  Classical.forall_intro (mem_locset_of_region reg2)
+
+let locset_of_region_liveness_tag_subset_locset_of_region_with_liveness
+  (r: HH.rid)
+: Lemma
+  (requires True)
+  (ensures (locset_of_region_liveness_tag r `TSet.subset` locset_of_region_with_liveness r))
+  [SMTPat (locset_of_region_liveness_tag r `TSet.subset` locset_of_region_with_liveness r)]
+= ()
+
+let locset_of_region_liveness_tag_disjoint_locset_of_region
+  (r1 r2: HH.rid)
+: Lemma
+  (requires True)
+  (ensures (locset_of_region_liveness_tag r1 `Modifies.locset_disjoint` locset_of_region r2))
+  [SMTPat (locset_of_region_liveness_tag r1 `Modifies.locset_disjoint` locset_of_region r2)]
+= Classical.forall_intro (mem_locset_of_region r2)
+
+private let test_1
+  (#t1 #t2: Type)
+  (reg: HH.rid)
+  (r1: reference t1)
+  (r2: reference t2)
+  (h1 h2 h3: mem)
+: Lemma
+  (requires (Modifies.modifies (locset_of_reference r1) h1 h2 /\ Modifies.modifies (locset_of_reference r2) h2 h3 /\ frameOf r1 == reg /\ frameOf r2 == reg))
+  (ensures (Modifies.modifies (locset_of_region reg) h1 h3))
+= ()
+
+let modifies_locset_of_reference_intro #a (h:mem) (x:reference a) (v:a) : Lemma
+  (requires (contains h x))
+  (ensures (contains h x
+	    /\ Modifies.modifies (locset_of_reference x) h (upd h x v)
+	    /\ sel (upd h x v) x == v ))
+  [SMTPat (upd h x v); SMTPatT (contains h x)]
+  = Modifies.modifies_intro (locset_of_reference x) h (upd h x v) (fun ty l c o g ->
+      Modifies.modifies_loc_refines_0 class (ObjectReference _ x) h (upd h x v) (fun o' _ -> ()) c o (g (Modifies.loc_of_object class (ObjectReference _ x)))
+    )
+
+let modifies_locset_of_reference_elim
+  #a
+  (x: reference a)
+  (s: Modifies.locset root_class)
+  (h h': mem)
+: Lemma
+  (requires (Modifies.modifies s h h' /\ Modifies.locset_disjoint (locset_of_reference x) s))
+  (ensures (contains h x ==> (contains h' x /\ sel h' x == sel h x)))
+= ()
+
+let modifies_locset_of_region_liveness_tag_elim
+  (x: HH.rid)
+  (s: Modifies.locset root_class)
+  (h h': mem)
+: Lemma
+  (requires (Modifies.modifies s h h' /\ Modifies.locset_disjoint (locset_of_region_liveness_tag x) s))
+  (ensures (live_region h x ==> live_region h' x))
+= ()
+
+let modifies_reference_elim
+  (#t: Type)
+  (r: reference t)
+  (s: Modifies.locset root_class)
+  (h h': mem)
+: Lemma
+  (requires (Modifies.modifies s h h' /\ Modifies.locset_disjoint (locset_of_reference r) s))
+  (ensures (contains h r ==> (contains h' r /\ sel h' r == sel h r)))
+  [SMTPatT (Modifies.modifies s h h'); SMTPatT (Modifies.locset_disjoint (locset_of_reference r) s)]
+= ()
